Simplify language/typed_prophet and language/wise_prophet.

theories/language/wise_prophet.v
@@ -9,154 +9,139 @@ From zebre.language Require Import
   notations
   diaframe.
 
-Record wise_strong_prophet `{zebre_G : !ZebreG Σ} := {
-  wise_strong_prophet_type : Type ;
-  wise_strong_prophet_to_val : wise_strong_prophet_type → val * val ;
+Class WiseStrongProphetG Σ `{zebre_G : !ZebreG Σ} prophet := {
+  #[local] wise_strong_prophet_G_full_G :: AgreeG Σ (leibnizO (list prophet.(typed_strong_prophet_type))) ;
+  #[local] wise_strong_prophet_G_past_G :: MonoListG Σ prophet.(typed_strong_prophet_type) ;
+}.
 
-  wise_strong_prophet_name : Type ;
-  #[global] wise_strong_prophet_name_eq_dec ::
-    EqDecision wise_strong_prophet_name ;
-  #[global] wise_strong_prophet_name_countable ::
-    Countable wise_strong_prophet_name ;
+Definition wise_strong_prophet_Σ prophet := #[
+  agree_Σ (leibnizO (list prophet.(typed_strong_prophet_type))) ;
+  mono_list_Σ prophet.(typed_strong_prophet_type)
+].
+#[global] Instance subG_wise_strong_prophet_Σ Σ `{zebre_G : !ZebreG Σ} prophet :
+  subG (wise_strong_prophet_Σ prophet) Σ →
+  WiseStrongProphetG Σ prophet.
+Proof.
+  solve_inG.
+Qed.
 
-  wise_strong_prophet_model : prophecy_id → wise_strong_prophet_name → list wise_strong_prophet_type → list wise_strong_prophet_type → iProp Σ ;
-  wise_strong_prophet_lb : wise_strong_prophet_name → list wise_strong_prophet_type → iProp Σ ;
+Section typed_strong_prophet.
+  Context (prophet : typed_strong_prophet).
+  Context `{wise_prophet_G : WiseStrongProphetG Σ prophet}.
 
-  #[global] wise_strong_prophet_model_timeless p γ past prophs ::
-    Timeless (wise_strong_prophet_model p γ past prophs) ;
-  #[global] wise_strong_prophet_lb_timeless γ lb ::
-    Timeless (wise_strong_prophet_lb γ lb) ;
-  #[global] wise_strong_prophet_lb_persistent γ lb ::
-    Persistent (wise_strong_prophet_lb γ lb) ;
+  Record wise_strong_prophet_name := {
+    wise_strong_prophet_name_full : gname ;
+    wise_strong_prophet_name_past : gname ;
+  }.
 
-  wise_strong_prophet_model_exclusive p γ1 past1 prophs1 γ2 past2 prophs2 :
+  #[global] Instance wise_strong_prophet_name_eq_dec : EqDecision wise_strong_prophet_name :=
+    ltac:(solve_decision).
+  #[global] Instance wise_strong_prophet_name_countable :
+    Countable wise_strong_prophet_name.
+  Proof.
+    pose encode γ := (
+      γ.(wise_strong_prophet_name_full),
+      γ.(wise_strong_prophet_name_past)
+    ).
+    pose decode := λ '(γ_full, γ_past), {|
+      wise_strong_prophet_name_full := γ_full ;
+      wise_strong_prophet_name_past := γ_past ;
+    |}.
+    refine (inj_countable' encode decode _). intros []. done.
+  Qed.
+
+  Definition wise_strong_prophet_model p γ past prophs : iProp Σ :=
+    agree_on γ.(wise_strong_prophet_name_full) (past ++ prophs) ∗
+    mono_list_auth γ.(wise_strong_prophet_name_past) (DfracOwn 1) past ∗
+    typed_strong_prophet_model prophet p prophs.
+
+  Definition wise_strong_prophet_lb γ lb : iProp Σ :=
+    ∃ past_lb,
+    agree_on γ.(wise_strong_prophet_name_full) (past_lb ++ lb) ∗
+    mono_list_lb γ.(wise_strong_prophet_name_past) past_lb.
+
+  #[global] Instance wise_strong_prophet_model_timeless p γ past prophs :
+    Timeless (wise_strong_prophet_model p γ past prophs).
+  Proof.
+    apply _.
+  Qed.
+  #[global] Instance wise_strong_prophet_lb_timeless γ lb :
+    Timeless (wise_strong_prophet_lb γ lb).
+  Proof.
+    apply _.
+  Qed.
+  #[global] Instance wise_strong_prophet_lb_persistent γ lb :
+    Persistent (wise_strong_prophet_lb γ lb).
+  Proof.
+    apply _.
+  Qed.
+
+  Lemma wise_strong_prophet_model_exclusive p γ1 past1 prophs1 γ2 past2 prophs2 :
     wise_strong_prophet_model p γ1 past1 prophs1 -∗
     wise_strong_prophet_model p γ2 past2 prophs2 -∗
-    False ;
+    False.
+  Proof.
+    iIntros "(_ & _ & Hmodel1) (_ & _ & Hmodel2)".
+    iApply (typed_strong_prophet_model_exclusive with "Hmodel1 Hmodel2").
+  Qed.
 
-  wise_strong_prophet_lb_get p γ past prophs :
+  Lemma wise_strong_prophet_lb_get p γ past prophs :
     wise_strong_prophet_model p γ past prophs -∗
-    wise_strong_prophet_lb γ prophs ;
-  wise_strong_prophet_model_lb_valid p γ past prophs lb :
+    wise_strong_prophet_lb γ prophs.
+  Proof.
+    iIntros "(#Hfull & Hpast_auth & Hmodel)".
+    iStep.
+    iApply (mono_list_lb_get with "Hpast_auth").
+  Qed.
+  Lemma wise_strong_prophet_model_lb_valid p γ past prophs lb :
     wise_strong_prophet_model p γ past prophs -∗
     wise_strong_prophet_lb γ lb -∗
-    ⌜∃ past1 past2, past = past1 ++ past2 ∧ lb = past2 ++ prophs⌝ ;
+    ⌜ ∃ past1 past2,
+      past = past1 ++ past2 ∧
+      lb = past2 ++ prophs
+    ⌝.
+  Proof.
+    iIntros "(#Hfull & Hpast_auth & Hmodel) (%past1 & #Hfull' & #Hpast_lb)".
+    iDestruct (agree_on_agree_L with "Hfull Hfull'") as %Hfull.
+    iDestruct (mono_list_lb_valid with "Hpast_auth Hpast_lb") as %(past2 & ->).
+    iPureIntro. rewrite -assoc in Hfull. naive_solver.
+  Qed.
 
-  wise_strong_prophet_wp_proph E :
+  Lemma wise_strong_prophet_wp_proph E :
     {{{ True }}}
       Proph @ E
     {{{ p γ prophs,
       RET #p;
       wise_strong_prophet_model p γ [] prophs
-    }}} ;
+    }}}.
+  Proof.
+    iIntros "%Φ _ HΦ".
+    iApply wp_fupd. wp_apply (typed_strong_prophet_wp_proph with "[//]") as "%p %prophs Hp".
+    iMod (agree_alloc (agree_G := wise_strong_prophet_G_full_G) prophs) as "(%γ_full & #Hfull)".
+    iMod (mono_list_alloc []) as "(%γ_past & Hpast_auth)".
+    set γ := {|
+      wise_strong_prophet_name_full := γ_full ;
+      wise_strong_prophet_name_past := γ_past ;
+    |}.
+    iApply ("HΦ" $! p γ).
+    iSteps.
+  Qed.
 
-  wise_strong_prophet_wp_resolve e v E p γ past prophs Φ :
+  Lemma wise_strong_prophet_wp_resolve e v E p γ past prophs Φ :
     Atomic e →
     to_val e = None →
     wise_strong_prophet_model p γ past prophs -∗
     WP e @ E {{ w,
       ∃ proph,
-      ⌜(w, v) = wise_strong_prophet_to_val proph⌝ ∗
+      ⌜(w, v) = prophet.(typed_strong_prophet_to_val) proph⌝ ∗
         ∀ prophs',
         ⌜prophs = proph :: prophs'⌝ -∗
         wise_strong_prophet_model p γ (past ++ [proph]) prophs' -∗
         Φ w
     }} -∗
-    WP Resolve e #p v @ E {{ Φ }} ;
-}.
-#[global] Arguments wise_strong_prophet _ {_} : assert.
-#[global] Arguments Build_wise_strong_prophet {_ _ _ _ _ _ _ _ _ _ _ _} _ _ _ _ _ : assert.
-#[global] Opaque wise_strong_prophet_model.
-#[global] Opaque wise_strong_prophet_lb.
-
-Class WiseStrongProphetG Σ `{zebre_G : !ZebreG Σ} spec := {
-  #[local] wise_strong_prophet_G_full_G :: AgreeG Σ (leibnizO (list spec.(typed_strong_prophet_spec_type))) ;
-  #[local] wise_strong_prophet_G_past_G :: MonoListG Σ spec.(typed_strong_prophet_spec_type) ;
-}.
-
-Definition wise_strong_prophet_Σ spec := #[
-  agree_Σ (leibnizO (list spec.(typed_strong_prophet_spec_type))) ;
-  mono_list_Σ spec.(typed_strong_prophet_spec_type)
-].
-#[global] Instance subG_wise_strong_prophet_Σ Σ `{zebre_G : !ZebreG Σ} spec :
-  subG (wise_strong_prophet_Σ spec) Σ →
-  WiseStrongProphetG Σ spec.
-Proof.
-  solve_inG.
-Qed.
-
-Section make_wise_prophet_G.
-  Context `{zebre_G : !ZebreG Σ} spec `{wise_prophet_G : !WiseStrongProphetG Σ spec}.
-
-  Definition make_wise_strong_prophet_typed_prophet :=
-    make_typed_strong_prophet spec.
-
-  Record make_wise_strong_prophet_name := {
-    make_wise_strong_prophet_name_full : gname ;
-    make_wise_strong_prophet_name_past : gname ;
-  }.
-  #[local] Instance make_wise_strong_prophet_name_eq_dec : EqDecision make_wise_strong_prophet_name :=
-    ltac:(solve_decision).
-  #[local] Instance make_wise_strong_prophet_name_countable :
-    Countable make_wise_strong_prophet_name.
+    WP Resolve e #p v @ E {{ Φ }}.
   Proof.
-    pose encode γ := (
-      γ.(make_wise_strong_prophet_name_full),
-      γ.(make_wise_strong_prophet_name_past)
-    ).
-    pose decode := λ '(γ_full, γ_past), {|
-      make_wise_strong_prophet_name_full := γ_full ;
-      make_wise_strong_prophet_name_past := γ_past ;
-    |}.
-    refine (inj_countable' encode decode _). intros []. done.
-  Qed.
-
-  Program Definition make_wise_strong_prophet := {|
-    wise_strong_prophet_type :=
-      spec.(typed_strong_prophet_spec_type) ;
-    wise_strong_prophet_to_val :=
-      spec.(typed_strong_prophet_spec_to_val) ;
-
-    wise_strong_prophet_model p γ past prophs := (
-      agree_on γ.(make_wise_strong_prophet_name_full) (past ++ prophs) ∗
-      mono_list_auth γ.(make_wise_strong_prophet_name_past) (DfracOwn 1) past ∗
-      make_wise_strong_prophet_typed_prophet.(typed_strong_prophet_model) p prophs
-    )%I ;
-    wise_strong_prophet_lb γ lb := (
-      ∃ past_lb,
-      agree_on γ.(make_wise_strong_prophet_name_full) (past_lb ++ lb) ∗
-      mono_list_lb γ.(make_wise_strong_prophet_name_past) past_lb
-    )%I ;
-  |}.
-  Next Obligation.
-    iIntros "* (_ & _ & Hmodel1) (_ & _ & Hmodel2)".
-    iApply (typed_strong_prophet_model_exclusive with "Hmodel1 Hmodel2").
-  Qed.
-  Next Obligation.
-    iIntros "* (#Hfull & Hpast_auth & Hmodel)".
-    iStep.
-    iApply (mono_list_lb_get with "Hpast_auth").
-  Qed.
-  Next Obligation.
-    iIntros "* (#Hfull & Hpast_auth & Hmodel) (%past1 & #Hfull' & #Hpast_lb)".
-    iDestruct (agree_on_agree_L with "Hfull Hfull'") as %Hfull.
-    iDestruct (mono_list_lb_valid with "Hpast_auth Hpast_lb") as %(past2 & ->).
-    iPureIntro. rewrite -assoc in Hfull. naive_solver.
-  Qed.
-  Next Obligation.
-    iIntros "* _ HΦ".
-    iApply wp_fupd. wp_apply (make_wise_strong_prophet_typed_prophet.(typed_strong_prophet_wp_proph) with "[//]") as "%p %prophs Hp".
-    iMod (agree_alloc (agree_G := wise_strong_prophet_G_full_G) prophs) as "(%γ_full & #Hfull)".
-    iMod (mono_list_alloc []) as "(%γ_past & Hpast_auth)".
-    set γ := {|
-      make_wise_strong_prophet_name_full := γ_full ;
-      make_wise_strong_prophet_name_past := γ_past ;
-    |}.
-    iApply ("HΦ" $! p γ).
-    iSteps.
-  Qed.
-  Next Obligation.
-    iIntros "* % % (#Hfull & Hpast_auth & Hmodel) HΦ".
+    iIntros "% % (#Hfull & Hpast_auth & Hmodel) HΦ".
     wp_apply (typed_strong_prophet_wp_resolve with "Hmodel"); first done.
     iApply wp_fupd. wp_apply (wp_wand with "HΦ") as "%w HΦ".
     iDestruct "HΦ" as "(%proph & % & HΦ)".
@@ -164,55 +149,118 @@ Section make_wise_prophet_G.
     iMod (mono_list_update_app [proph] with "Hpast_auth") as "Hpast_auth".
     iIntros "!> %prophs' -> Hp".
     iApply ("HΦ" with "[//]").
-    list_simplifier. iSteps.
+    rewrite (assoc _ _ [_]). iSteps.
   Qed.
-End make_wise_prophet_G.
+End typed_strong_prophet.
 
-Record wise_prophet `{zebre_G : !ZebreG Σ} := {
-  wise_prophet_type : Type ;
-  wise_prophet_to_val : wise_prophet_type → val ;
+#[global] Opaque wise_strong_prophet_model.
+#[global] Opaque wise_strong_prophet_lb.
 
-  wise_prophet_name : Type ;
-  #[global] wise_prophet_name_eq_dec ::
-    EqDecision wise_prophet_name ;
-  #[global] wise_prophet_name_countable ::
-    Countable wise_prophet_name ;
+Class WiseProphetG Σ `{zebre_G : !ZebreG Σ} prophet := {
+  #[local] wise_prophet_G_full_G :: AgreeG Σ (leibnizO (list (val * prophet.(typed_prophet_type)))) ;
+  #[local] wise_prophet_G_past_G :: MonoListG Σ (val * prophet.(typed_prophet_type)) ;
+}.
 
-  wise_prophet_model : prophecy_id → wise_prophet_name → list wise_prophet_type → list wise_prophet_type → iProp Σ ;
-  wise_prophet_lb : wise_prophet_name → list wise_prophet_type → iProp Σ ;
+Definition wise_prophet_Σ prophet := #[
+  agree_Σ (leibnizO (list (val * prophet.(typed_prophet_type)))) ;
+  mono_list_Σ (val * prophet.(typed_prophet_type))
+].
+#[global] Instance subG_wise_prophet_Σ Σ `{zebre_G : !ZebreG Σ} prophet :
+  subG (wise_prophet_Σ prophet) Σ →
+  WiseProphetG Σ prophet.
+Proof.
+  solve_inG.
+Qed.
 
-  #[global] wise_prophet_model_timeless p γ past prophs ::
-    Timeless (wise_prophet_model p γ past prophs) ;
-  #[global] wise_prophet_lb_timeless γ lb ::
-    Timeless (wise_prophet_lb γ lb) ;
-  #[global] wise_prophet_lb_persistent γ lb ::
-    Persistent (wise_prophet_lb γ lb) ;
+Section typed_prophet.
+  Context (prophet : typed_prophet).
+  Context `{wise_prophet_G : WiseProphetG Σ prophet}.
 
-  wise_prophet_model_exclusive p γ1 past1 prophs1 γ2 past2 prophs2 :
+  Definition wise_prophet_name :=
+    wise_strong_prophet_name.
+  Implicit Types γ : wise_prophet_name.
+
+  #[local] Instance wise_prophet_strong_prophet_G :
+    WiseStrongProphetG Σ prophet.
+  Proof.
+    split; apply _.
+  Qed.
+
+  Definition wise_prophet_model p γ past prophs : iProp Σ :=
+    ∃ spast sprophs,
+    ⌜past = spast.*2⌝ ∗
+    ⌜prophs = sprophs.*2⌝ ∗
+    wise_strong_prophet_model prophet p γ spast sprophs.
+
+  Definition wise_prophet_lb γ lb : iProp Σ :=
+    ∃ slb,
+    ⌜lb = slb.*2⌝ ∗
+    wise_strong_prophet_lb prophet γ slb.
+
+  #[global] Instance wise_prophet_model_timeless p γ past prophs :
+    Timeless (wise_prophet_model p γ past prophs).
+  Proof.
+    apply _.
+  Qed.
+  #[global] Instance wise_prophet_lb_timeless γ lb :
+    Timeless (wise_prophet_lb γ lb).
+  Proof.
+    apply _.
+  Qed.
+  #[global] Instance wise_prophet_lb_persistent γ lb :
+    Persistent (wise_prophet_lb γ lb).
+  Proof.
+    apply _.
+  Qed.
+
+  Lemma wise_prophet_model_exclusive p γ1 past1 prophs1 γ2 past2 prophs2 :
     wise_prophet_model p γ1 past1 prophs1 -∗
     wise_prophet_model p γ2 past2 prophs2 -∗
-    False ;
+    False.
+  Proof.
+    iIntros "(%spast1 & %sprophs1 & _ & _ & Hmodel1) (%spast2 & %sprophs2 & _ & _ & Hmodel2)".
+    iApply (wise_strong_prophet_model_exclusive with "Hmodel1 Hmodel2").
+  Qed.
 
-  wise_prophet_lb_get p γ past prophs :
+  Lemma wise_prophet_lb_get p γ past prophs :
     wise_prophet_model p γ past prophs -∗
-    wise_prophet_lb γ prophs ;
-  wise_prophet_model_lb_valid p γ past prophs lb :
+    wise_prophet_lb γ prophs.
+  Proof.
+    iIntros "(%spast & %sprophs & -> & -> & Hmodel)".
+    iStep.
+    iApply (wise_strong_prophet_lb_get with "Hmodel").
+  Qed.
+  Lemma wise_prophet_model_lb_valid p γ past prophs lb :
     wise_prophet_model p γ past prophs -∗
     wise_prophet_lb γ lb -∗
-    ⌜∃ past1 past2, past = past1 ++ past2 ∧ lb = past2 ++ prophs⌝ ;
+    ⌜ ∃ past1 past2,
+      past = past1 ++ past2 ∧
+      lb = past2 ++ prophs
+    ⌝.
+  Proof.
+    iIntros "(%spast & %sprophs & -> & -> & Hmodel) (%slb & -> & Hlb)".
+    iDestruct (wise_strong_prophet_model_lb_valid with "Hmodel Hlb") as "(%spast1 & %spast2 & -> & ->)".
+    list_simplifier. iSteps.
+  Qed.
 
-  wise_prophet_wp_proph E :
+  Lemma wise_prophet_wp_proph E :
     {{{ True }}}
       Proph @ E
     {{{ p γ prophs,
       RET #p;
       wise_prophet_model p γ [] prophs
-    }}} ;
+    }}}.
+  Proof.
+    iIntros "%Φ _ HΦ".
+    wp_apply (wise_strong_prophet_wp_proph prophet with "[//]") as "%p %γ %sprophs Hmodel".
+    iApply "HΦ".
+    iExists [], sprophs. iSteps.
+  Qed.
 
-  wise_prophet_wp_resolve proph e v E p γ past prophs Φ :
+  Lemma wise_prophet_wp_resolve proph e v E p γ past prophs Φ :
     Atomic e →
     to_val e = None →
-    v = wise_prophet_to_val proph →
+    v = prophet.(typed_prophet_to_val) proph →
     wise_prophet_model p γ past prophs -∗
     WP e @ E {{ w,
       ∀ prophs',
@@ -220,101 +268,16 @@ Record wise_prophet `{zebre_G : !ZebreG Σ} := {
       wise_prophet_model p γ (past ++ [proph]) prophs' -∗
       Φ w
     }} -∗
-    WP Resolve e #p v @ E {{ Φ }} ;
-}.
-#[global] Arguments wise_prophet _ {_} : assert.
-#[global] Arguments Build_wise_prophet {_ _ _ _ _ _ _ _ _ _ _ _} _ _ _ _ _ : assert.
-#[global] Opaque wise_prophet_model.
-#[global] Opaque wise_prophet_lb.
-
-Class WiseProphetG Σ `{zebre_G : !ZebreG Σ} spec := {
-  #[local] wise_prophet_G_full_G :: AgreeG Σ (leibnizO (list (val * spec.(typed_prophet_spec_type)))) ;
-  #[local] wise_prophet_G_past_G :: MonoListG Σ (val * spec.(typed_prophet_spec_type)) ;
-}.
-
-Definition wise_prophet_Σ spec := #[
-  agree_Σ (leibnizO (list (val * spec.(typed_prophet_spec_type)))) ;
-  mono_list_Σ (val * spec.(typed_prophet_spec_type))
-].
-#[global] Instance subG_wise_prophet_Σ Σ `{zebre_G : !ZebreG Σ} spec :
-  subG (wise_prophet_Σ spec) Σ →
-  WiseProphetG Σ spec.
-Proof.
-  solve_inG.
-Qed.
-
-Section make_wise_prophet.
-  Context `{zebre_G : !ZebreG Σ} spec `{wise_prophet_G : !WiseProphetG Σ spec}.
-
-  #[local] Program Definition make_wise_prophet_strong_prophet_spec := {|
-    typed_strong_prophet_spec_type :=
-      val * spec.(typed_prophet_spec_type) ;
-    typed_strong_prophet_spec_of_val w v :=
-      match spec.(typed_prophet_spec_of_val) v with
-      | None => None
-      | Some proph => Some (w, proph)
-      end ;
-    typed_strong_prophet_spec_to_val '(w, proph) :=
-      (w, spec.(typed_prophet_spec_to_val) proph) ;
-  |}.
-  Next Obligation.
-    intros (w & proph) _w v [= -> ->].
-    erewrite spec.(typed_prophet_spec_of_to_val); done.
-  Qed.
-
-  #[local] Instance make_wise_prophet_strong_prophet_G :
-    WiseStrongProphetG Σ make_wise_prophet_strong_prophet_spec.
+    WP Resolve e #p v @ E {{ Φ }}.
   Proof.
-    split; apply _.
-  Qed.
-
-  #[local] Definition make_wise_prophet_strong_prophet :=
-    make_wise_strong_prophet make_wise_prophet_strong_prophet_spec.
-
-  Program Definition make_wise_prophet := {|
-    wise_prophet_type :=
-      spec.(typed_prophet_spec_type) ;
-    wise_prophet_to_val :=
-      spec.(typed_prophet_spec_to_val) ;
-
-    wise_prophet_model p γ past prophs := (
-      ∃ spast sprophs,
-      ⌜past = spast.*2⌝ ∗
-      ⌜prophs = sprophs.*2⌝ ∗
-      make_wise_prophet_strong_prophet.(wise_strong_prophet_model) p γ spast sprophs
-    )%I ;
-    wise_prophet_lb γ lb := (
-      ∃ slb,
-      ⌜lb = slb.*2⌝ ∗
-      make_wise_prophet_strong_prophet.(wise_strong_prophet_lb) γ slb
-    )%I ;
-  |}.
-  Next Obligation.
-    iIntros "* (%spast1 & %sprophs1 & _ & _ & Hmodel1) (%spast2 & %sprophs2 & _ & _ & Hmodel2)".
-    iApply (wise_strong_prophet_model_exclusive with "Hmodel1 Hmodel2").
-  Qed.
-  Next Obligation.
-    iIntros "* (%spast & %sprophs & -> & -> & Hmodel)".
-    iStep.
-    iApply (wise_strong_prophet_lb_get with "Hmodel").
-  Qed.
-  Next Obligation.
-    iIntros "* (%spast & %sprophs & -> & -> & Hmodel) (%slb & -> & Hlb)".
-    iDestruct (wise_strong_prophet_model_lb_valid with "Hmodel Hlb") as "(%spast1 & %spast2 & -> & ->)".
-    list_simplifier. iSteps.
-  Qed.
-  Next Obligation.
-    iIntros "* _ HΦ".
-    wp_apply (make_wise_prophet_strong_prophet.(wise_strong_prophet_wp_proph) with "[//]") as "%p %γ %sprophs Hmodel".
-    iApply "HΦ". iExists [], sprophs.
-    iSteps.
-  Qed.
-  Next Obligation.
-    iIntros "*" (? ? ->) "(%spast & %sprophs & -> & -> & Hmodel) HΦ".
+    iIntros (? ? ->) "(%spast & %sprophs & -> & -> & Hmodel) HΦ".
     wp_apply (wise_strong_prophet_wp_resolve with "Hmodel"); first done.
     wp_apply (wp_wand with "HΦ") as "%w HΦ".
     iExists (w, proph). iSplit; first iSteps. iIntros "%sprophs' -> Hmodel".
     iApply ("HΦ" with "[//]"). iExists (spast ++ [(w, proph)]), sprophs'. iFrame.
     list_simplifier. iSteps.
   Qed.
-End make_wise_prophet.
+End typed_prophet.
+
+#[global] Opaque wise_prophet_model.
+#[global] Opaque wise_prophet_lb.
